proof: refine the definition for tuples

policy_proof/coq/data_model.v
@@ -278,12 +278,9 @@ End Policy.
 Module Cell.
 
 (* A cell that does not carry policies. *)
-Definition clean_cell: Set := basic_type % type.
 (* A cell that carries policies . *)
-Definition cell: Set := (clean_cell * Policy.policy) % type.
-Definition cell_denote (c: cell): Set := (type_to_coq_type (fst c) * Policy.policy) % type.
-
-Definition cell_inject_policy (c: clean_cell) (p: Policy.policy): cell := (c, p).
+Definition cell: Set := basic_type % type.
+Definition cell_denote (c: cell): Set := (type_to_coq_type c) % type.
 
 Global Instance cell_denote_eq_propers:
   Proper (equiv ==> equiv) (cell_denote).
@@ -297,7 +294,6 @@ Module Tuple.
 
 (* A tuple is a list of cells of different values. *)
 Definition tuple_type: Set := (list Cell.cell)%type.
-Definition tuple_type_np: Set := (list Cell.clean_cell)%type.
 
 (* A tuple is, in essence, an interpretation of abstract values to their
 concrete values. Thus it is a dependent type of `tuple_type`. We also
@@ -305,10 +301,10 @@ make it a recursive type, so that we can build types of arbitrary length. *)
 Fixpoint tuple (ty: tuple_type): Set :=
   match ty with
   | nil => unit
-  | c :: t' => Cell.cell_denote c * tuple t'
+  | bt :: t' => ((type_to_coq_type bt) * Policy.policy) * tuple t'
   end%type.
 
-Fixpoint tuple_np (ty: tuple_type_np): Set :=
+Fixpoint tuple_np (ty: tuple_type): Set :=
   match ty with
     | nil => unit
     | bt :: t' => (type_to_coq_type bt) * tuple_np t'
@@ -317,34 +313,22 @@ Fixpoint tuple_np (ty: tuple_type_np): Set :=
 Fixpoint tuple_value_lt (ty: tuple_type): forall (lhs rhs: tuple ty), Prop :=
   match ty return forall (lhs rhs: tuple ty), Prop with
     | nil => fun _ _ => False
-    | (bt, _) :: t' => fun lhs rhs => lt (fst (fst lhs)) (fst (fst rhs)) \/
+    | _ :: t' => fun lhs rhs => lt (fst (fst lhs)) (fst (fst rhs)) \/
       (fst (fst lhs)) == (fst (fst rhs)) /\ tuple_value_lt t' (snd lhs) (snd rhs)
   end.
 
 Fixpoint tuple_total_lt (ty: tuple_type): forall (lhs rhs: tuple ty), Prop :=
   match ty return forall (lhs rhs: tuple ty), Prop with
     | nil => fun _ _ => False
-    | (bt, _) :: t' => fun lhs rhs => lt (fst lhs) (fst rhs) \/
+    | _ :: t' => fun lhs rhs => lt (fst lhs) (fst rhs) \/
       (fst lhs) == (fst rhs) /\ tuple_total_lt t' (snd lhs) (snd rhs)
   end.
 
-(* todo. *)
-Fixpoint inject_policy (p: list Policy.policy) (ty: tuple_type_np): tuple_type :=
-  match p, ty with
-    | nil, nil => nil
-    | p' :: p'', bt :: t' => (bt, p') :: inject_policy p'' t'
-    | _, _ => nil
-  end.
-
-(* Revoves policies. *)
-Definition extract_types (ty: tuple_type): tuple_type_np :=
-  List.map (fun x => fst x) ty.
-
 (* A tuple type is a list of basic types. *)
 
-Definition example_tuple_ty : tuple_type := (StringType, Policy.policy_bot) :: (BoolType, Policy.policy_bot) :: nil.
+Definition example_tuple_ty : tuple_type := StringType :: BoolType :: nil.
 Definition example_tuple: tuple example_tuple_ty := (("abcd"%string, Policy.policy_bot), ((true, Policy.policy_bot), tt)).
-Definition example_tuple_ty' : tuple_type := (IntegerType, Policy.policy_bot) :: nil.
+Definition example_tuple_ty' : tuple_type := IntegerType :: nil.
 Definition example_tuple' : tuple example_tuple_ty' := ((1, Policy.policy_bot), tt).
 Definition example_tuple'' : tuple (example_tuple_ty' ++ example_tuple_ty) := 
   ((1, Policy.policy_bot),
@@ -358,14 +342,14 @@ Lemma tuple_cast: forall (ty1 ty2: tuple_type) (f: tuple_type -> Set),
 Proof.
   intros.
   rewrite H0 in H.
-  auto. 
+  auto.
 Qed.
 
 (* A tuple type is a list of basic types. *)
 Fixpoint tuple_type_eq (ty1 ty2: tuple_type) : bool :=
   match ty1, ty2 with
     | nil, nil => true
-    | (bt1, _) :: t1', (bt2, _) :: t2' => andb (type_matches bt1 bt2) (tuple_type_eq t1' t2')
+    | bt1 :: t1', bt2 :: t2' => andb (type_matches bt1 bt2) (tuple_type_eq t1' t2')
     | _, _ => false
   end.
 
@@ -390,44 +374,44 @@ Qed.
 Fixpoint tuple_value_eq (ty: tuple_type): forall (lhs rhs: tuple ty), Prop :=
   match ty return (forall (lhs rhs: tuple ty), Prop) with
     | nil => fun _ _ => True
-    | (h, p) :: tl => fun lhs rhs => 
+    | _ :: tl => fun lhs rhs => 
       (fst (fst lhs)) == (fst (fst rhs)) /\ tuple_value_eq tl (snd lhs) (snd rhs)
   end. 
 
 Fixpoint tuple_total_eq (ty: tuple_type): forall (lhs rhs: tuple ty), Prop :=
   match ty return (forall (lhs rhs: tuple ty), Prop) with
     | nil => fun _ _ => True
-    | (h, p) :: tl => fun lhs rhs => 
+    | _ :: tl => fun lhs rhs => 
       (fst lhs) == (fst rhs) /\ tuple_total_eq tl (snd lhs) (snd rhs)
-  end. 
+  end.
 
 Global Instance tuple_value_eq_eqv (ty: tuple_type): Equivalence (tuple_value_eq ty).
   (* Note that `Equivalence` is a class. *)
   constructor.
   - unfold Reflexive.
-    intros. induction ty; intuition auto with *. destruct a; destruct c; simpl in *; auto. split; try reflexivity; auto.
+    intros. induction ty; intuition auto with *. destruct a; simpl in *; auto. split; try reflexivity; auto.
   - unfold Symmetric.
-    intros. induction ty; intuition auto with *. destruct a; destruct c; simpl in *; intuition auto with *.
+    intros. induction ty; intuition auto with *. destruct a; simpl in *; intuition auto with *.
   - unfold Transitive.
-    induction ty; intuition auto with *. destruct a; destruct c; simpl in *; intuition auto with *.
+    induction ty; intuition auto with *. destruct a; simpl in *; intuition auto with *.
     specialize (IHty _ _ _ H2 H3). assumption.
     eapply transitivity; eauto.
     specialize (IHty _ _ _ H2 H3). assumption.
     eapply transitivity; eauto.
-    specialize (IHty _ _ _ H2 H3). assumption.    
+    specialize (IHty _ _ _ H2 H3). assumption.
 Defined.
 
 Definition tuple_total_eq_eqv (ty: tuple_type): Equivalence (tuple_total_eq ty).
   (* Note that `Equivalence` is a class. *)
   split.
   - unfold Reflexive.
-    intros. induction ty. intuition auto with *. destruct a; destruct c; simpl in *; intuition auto with *;
+    intros. induction ty. intuition auto with *. destruct a; simpl in *; intuition auto with *;
     unfold pair_eq; auto with *.
   - unfold Symmetric.
-    intros. induction ty. intuition auto with *. destruct a; destruct c; simpl in *; intuition auto with *;
+    intros. induction ty. intuition auto with *. destruct a; simpl in *; intuition auto with *;
     unfold pair_eq in *; intuition auto with *.
   - unfold Transitive.
-    intros. induction ty. auto. destruct a. destruct c.
+    intros. induction ty. auto. destruct a.
     simpl in *. intuition; unfold pair_eq in *; intuition; auto with *.
       + rewrite H0. assumption.
       + rewrite H4. assumption.
@@ -463,8 +447,8 @@ refine (
     tuple ty -> tuple ((nth ty n extract) :: nil) :=
       match ty as ty', n as n' return ty = ty' -> n = n' -> 
             forall (extract: n' < length ty'), tuple ty' -> tuple ((nth ty' n' extract) :: nil) with
-        | (bt, p) :: l', 0 => fun _ _ _ t => ((fst t), tt)
-        | (bt, p) :: l', S n' => fun _ _ _ t => nth_col_tuple' l' n' _ (snd t)
+        |_  :: l', 0 => fun _ _ _ t => ((fst t), tt)
+        | _ :: l', S n' => fun _ _ _ t => nth_col_tuple' l' n' _ (snd t)
         | _, _ => fun _ _ _ => fun _ => False_rec _ _
       end (refl_equal _) (refl_equal _)).
 Proof.
@@ -481,7 +465,7 @@ Qed.
 (* Without `policy` extracted! *)
 Definition nth_np: forall (ty: tuple_type) (n: nat) (extract: n < length ty), basic_type.
   intros.
-  exact (fst (nth ty n extract)).
+  exact (nth ty n extract).
 Defined.
 
 (* Without `policy` extracted! *)
@@ -491,8 +475,8 @@ refine (
     tuple ty -> tuple_np ((nth_np ty n extract) :: nil) :=
       match ty as ty', n as n' return ty = ty' -> n = n' -> 
             forall (extract: n' < length ty'), tuple ty' -> tuple_np ((nth_np ty' n' extract) :: nil) with
-        | (bt, p) :: l', 0 => fun _ _ _ t => ((fst (fst t)), tt)
-        | (bt, p) :: l', S n' => fun _ _ _ t => nth_col_tuple_np' l' n' _ (snd t)
+        | _ :: l', 0 => fun _ _ _ t => ((fst (fst t)), tt)
+        | _ :: l', S n' => fun _ _ _ t => nth_col_tuple_np' l' n' _ (snd t)
         | _, _ => fun _ _ _ => fun _ => False_rec _ _
       end (refl_equal _) (refl_equal _)).
 simpl in *. lia.
@@ -515,7 +499,7 @@ Definition tuple_value_compare: forall (ty: tuple_type) (lhs rhs: tuple ty),
 Proof.
   intros. induction ty.
   - apply OrderedType.EQ. simpl. auto.
-  - destruct a; destruct c.
+  - destruct a.
     + simpl in lhs. simpl in rhs. destruct (cmp (fst (fst lhs)) (fst (fst rhs))).
       * apply OrderedType.LT. simpl. auto.
       * destruct (IHty (snd lhs) (snd rhs)).
@@ -543,7 +527,7 @@ Qed.
 Global Instance tuple_value_lt_trans (ty: tuple_type): Transitive (tuple_value_lt ty).
   unfold Transitive. induction ty.
   + intros. auto.
-  + destruct a; destruct c. simpl in *.
+  + destruct a; simpl in *.
     (* Integer. *)
     intuition auto with *. left. eapply transitivity; eauto. simpl in *.
     left. rewrite H0 in H1. assumption.
@@ -571,7 +555,7 @@ Defined.
 Global Instance tuple_total_lt_trans (ty: tuple_type): Transitive (tuple_total_lt ty).
   unfold Transitive. induction ty.
   - intros. auto.
-  - destruct a; destruct c. 
+  - destruct a. 
     + simpl in *. unfold pair_lt, pair_eq in *. intuition.
       * left. left. eapply transitivity; eauto.
       * left. left. rewrite H in H0. assumption.
@@ -646,7 +630,7 @@ refine(
   - intros. simpl. unfold complement.
     induction ty.
     + simpl in H. exfalso. assumption.
-    + intros. destruct a; destruct c; simpl in *; unfold pair_lt, pair_eq in *; intuition.
+    + intros. destruct a; simpl in *; unfold pair_lt, pair_eq in *; intuition.
       * rewrite H0 in H. apply neq in H. auto with *.
       * rewrite H3 in H4. apply neq in H4. auto with *.
       * specialize (IHty _ _ H4 H2). assumption.
@@ -661,7 +645,7 @@ refine(
   
   - induction ty.
     + intros. apply OrderedType.EQ. apply unit_eq_equiv. auto.
-    + intros. destruct a; destruct c.
+    + intros. destruct a.
       * destruct (cmp (fst lhs) (fst rhs)).
         -- apply OrderedType.LT. simpl. auto.
         -- destruct (IHty (snd lhs) (snd rhs)).
@@ -702,7 +686,7 @@ refine(
   simpl. unfold complement. intros.
   induction ty.
   - simpl in H. exfalso. assumption.
-  - destruct a; destruct c; simpl in *; unfold pair_lt, pair_eq in *; intuition.
+  - destruct a; simpl in *; unfold pair_lt, pair_eq in *; intuition.
     * rewrite H1 in H0. unfold nat_lt in H0. auto with *.
     * specialize (IHty _ _ H3 H2). assumption.
     * unfold bool_lt in H0. destruct H0. rewrite H in H1. rewrite H0 in H1. inversion H1.
@@ -712,7 +696,7 @@ refine(
 
   - intros. induction ty.
     * apply OrderedType.EQ. simpl. red. auto.
-    * destruct a; destruct c; destruct (cmp (fst (fst lhs)) (fst (fst rhs))).
+    * destruct a; destruct (cmp (fst (fst lhs)) (fst (fst rhs))).
       + apply OrderedType.LT. simpl. auto.
       + destruct (IHty (snd lhs) (snd rhs)).
         apply OrderedType.LT. simpl. auto.
@@ -737,8 +721,11 @@ Defined.
 
 Definition example_tuple_lhs : tuple example_tuple_ty := (("abcd"%string, Policy.policy_bot), ((true, Policy.policy_bot), tt)).
 Definition example_tuple_rhs : tuple example_tuple_ty := (("abcd"%string, Policy.policy_bot), ((true, Policy.policy_bot), tt)).
-
-Example example_tuple_total_eq: tuple_total_eq example_tuple_ty example_tuple_lhs example_tuple_lhs.
+Set Printing Constructor.
+Set Printing Coercions.
+Set Printing Implicit.
+Set Printing Projections.
+Example example_tuple_total_eq: tuple_total_eq example_tuple_ty example_tuple_lhs example_tuple_rhs.
 Proof.
   simpl. repeat split; simpl; reflexivity.
 Qed.
@@ -755,16 +742,6 @@ Definition config:= (Policy.label_lookup, privacy, unit)%type.
 End Configuration.
 
 Ltac str_eq:= auto; simpl in *; unfold char_eq in *; unfold char_lt in *; lia.
-
-Require Import finite_bags.
-
-Module Relation.
-
-Definition relation: Set := fbag Tuple.tuple_type.
-
-(* Global Instance relation_is_fbag: FiniteBag Tuple.tuple_type. *)
-
-End Relation.
 
 Section Facts.
   Context {ty: Tuple.tuple_type}.
