policy_proof/coq/relation.v
@@ -1,0 +1,26 @@
+Require Import Nat.
+Require Import List.
+Require Import String.
+
+Require Import data_model.
+Require Import ordering.
+Require Import finite_bags.
+Require Import types.
+
+(** 
+  [relation_np] is a function that takes a tuple type [ty] as an argument and returns a finite bag (fbag) of tuples of type [ty]. 
+  This function is used to define a relation in the context of a database or a similar data structure where relations are represented as collections of tuples.
+  Note: this will make tuple ignorant of the policy.
+  @param ty  The type of the tuples that will be stored in the relation.
+  @return    A finite bag (fbag) of tuples of type [ty].
+*)
+Definition relation_np (ty: Tuple.tuple_type) := fbag (Tuple.tuple ty).
+
+(** 
+  [relation] is a function that takes a tuple type [ty] as an argument and returns a finite bag (fbag) of tuples of type [ty]. 
+  This function is used to define a relation in the context of a database or a similar data structure where relations are represented as collections of tuples.
+
+  @param ty  The type of the tuples that will be stored in the relation.
+  @return    A finite bag (fbag) of tuples of type [ty].
+*)
+Definition relation (ty: Tuple.tuple_type) := fbag (Tuple.tuple ty).
